src/program_proof/rsm/distx_txnlog.v
@@ -9,16 +9,17 @@ Section program.
   Definition command_to_val (c : command) : val.
   Admitted.
   
-  Definition is_txnlog (log : loc) (gid : groupid) (γ : distx_names) : iProp Σ.
+  Definition own_txnlog (log : loc) (gid : groupid) (γ : distx_names) : iProp Σ.
   Admitted.
 
   Theorem wp_TxnLog__Lookup (log : loc) (lsn : u64) (gid : groupid) γ :
-    is_txnlog log gid γ -∗
-    {{{ True }}}
+    ⊢
+    {{{ own_txnlog log gid γ }}}
     <<< ∀∀ l, clog_half γ gid l >>>
       TxnLog__Lookup #log #lsn @ ↑txnlogN
     <<< ∃∃ l', clog_half γ gid l' >>>
     {{{ (c : command) (ok : bool), RET (command_to_val c, #ok);
+        own_txnlog log gid γ ∗
         ⌜if ok then l' !! (uint.nat lsn) = Some c else True⌝
     }}}.
   Proof.
@@ -28,12 +29,12 @@ Section program.
   Admitted.
 
   Theorem wp_TxnLog__SubmitAbort (log : loc) (ts : u64) (gid : groupid) γ :
-    is_txnlog log gid γ -∗
-    {{{ True }}}
+    ⊢
+    {{{ own_txnlog log gid γ }}}
     <<< ∀∀ vs, cpool_half γ gid vs >>>
       TxnLog__SubmitAbort #log #ts @ ↑txnlogN
     <<< cpool_half γ gid ({[CmdAbt (uint.nat ts)]} ∪ vs) >>>
-    {{{ (lsn : u64) (term : u64), RET (#lsn, #term); True }}}.
+    {{{ (lsn : u64) (term : u64), RET (#lsn, #term); own_txnlog log gid γ }}}.
   Proof.
     (*@ func (log *TxnLog) SubmitAbort(ts uint64) (uint64, uint64) {            @*)
     (*@     // TODO: marshalling a abort command                                @*)
@@ -43,12 +44,12 @@ Section program.
   Admitted.
 
   Theorem wp_TxnLog__SubmitCommit (log : loc) (ts : u64) (gid : groupid) γ :
-    is_txnlog log gid γ -∗
-    {{{ True }}}
+    ⊢
+    {{{ own_txnlog log gid γ }}}
     <<< ∀∀ vs, cpool_half γ gid vs >>>
       TxnLog__SubmitCommit #log #ts @ ↑txnlogN
     <<< cpool_half γ gid ({[CmdCmt (uint.nat ts)]} ∪ vs) >>>
-    {{{ (lsn : u64) (term : u64), RET (#lsn, #term); True }}}.
+    {{{ (lsn : u64) (term : u64), RET (#lsn, #term); own_txnlog log gid γ }}}.
   Proof.
     (*@ func (log *TxnLog) SubmitCommit(ts uint64) (uint64, uint64) {           @*)
     (*@     // TODO: marshalling a commit command                               @*)
@@ -60,12 +61,12 @@ Section program.
   Theorem wp_TxnLog__SubmitPrepare
     (log : loc) (ts : u64) (wrs : Slice.t)
     (wrsM : dbmap) (gid : groupid) γ :
-    is_txnlog log gid γ -∗
-    {{{ True (* TODO: slice ownership *) }}}
+    ⊢
+    {{{ own_txnlog log gid γ (* TODO: slice ownership *) }}}
     <<< ∀∀ vs, cpool_half γ gid vs >>>
       TxnLog__SubmitPrepare #log #ts (to_val wrs) @ ↑txnlogN
     <<< cpool_half γ gid ({[CmdPrep (uint.nat ts) wrsM]} ∪ vs) >>>
-    {{{ (lsn : u64) (term : u64), RET (#lsn, #term); True }}}.
+    {{{ (lsn : u64) (term : u64), RET (#lsn, #term); own_txnlog log gid γ }}}.
   Proof.
     (* some mixcode bug when function takes a slice *)
     (*@     // TODO: marshalling a prepare command                              @*)
@@ -76,12 +77,12 @@ Section program.
 
   Theorem wp_TxnLog__SubmitRead
     (log : loc) (ts : u64) (key : string) (gid : groupid) γ :
-    is_txnlog log gid γ -∗
-    {{{ True }}}
+    ⊢
+    {{{ own_txnlog log gid γ }}}
     <<< ∀∀ vs, cpool_half γ gid vs >>>
       TxnLog__SubmitRead #log #ts #(LitString key) @ ↑txnlogN
     <<< cpool_half γ gid ({[CmdRead (uint.nat ts) key]} ∪ vs) >>>
-    {{{ (lsn : u64) (term : u64), RET (#lsn, #term); True }}}.
+    {{{ (lsn : u64) (term : u64), RET (#lsn, #term); own_txnlog log gid γ }}}.
   Proof.
     (*@ func (log *TxnLog) SubmitRead(ts uint64, key string) (uint64, uint64) { @*)
     (*@     // TODO: marshalling a read command                                 @*)
@@ -93,10 +94,12 @@ Section program.
   Theorem wp_TxnLog__WaitUntilSafe
     (log : loc) (lsn : u64) (term : u64) (c : command) (gid : groupid) γ :
     cmd_receipt γ gid (uint.nat lsn) (uint.nat term) c -∗
-    is_txnlog log gid γ -∗
-    {{{ True }}}
+    {{{ own_txnlog log gid γ }}}
       TxnLog__WaitUntilSafe #log #lsn #term
-    {{{ (ok : bool), RET #ok; ∃ l, clog_lb γ gid l ∧ ⌜l !! (uint.nat lsn) = Some c⌝ }}}.
+    {{{ (ok : bool), RET #ok;
+        own_txnlog log gid γ ∗
+        ∃ l, clog_lb γ gid l ∧ ⌜l !! (uint.nat lsn) = Some c⌝
+    }}}.
   Proof.
     (*@ func (log *TxnLog) WaitUntilSafe(lsn uint64, term uint64) bool {        @*)
     (*@     // TODO: invoke paxos.WaitUntilSafe(lsn, term)                      @*)
